<?xml version="1.0"?>
<rdf:RDF xmlns="http://purl.obolibrary.org/obo/uo.owl#"
     xml:base="http://purl.obolibrary.org/obo/uo.owl"
     xmlns:owl="http://www.w3.org/2002/07/owl#"
     xmlns:rdf="http://www.w3.org/1999/02/22-rdf-syntax-ns#"
     xmlns:xml="http://www.w3.org/XML/1998/namespace"
     xmlns:xsd="http://www.w3.org/2001/XMLSchema#"
     xmlns:rdfs="http://www.w3.org/2000/01/rdf-schema#"
     xmlns:oboInOwl="http://www.geneontology.org/formats/oboInOwl#">
    <owl:Ontology rdf:about="http://purl.obolibrary.org/obo/uo.owl">
        <owl:versionIRI rdf:resource="http://purl.obolibrary.org/obo/uo/releases/2023-05-25/uo.owl"/>
    </owl:Ontology>
    


    <!-- 
    ///////////////////////////////////////////////////////////////////////////////////////
    //
    // Annotation properties
    //
    ///////////////////////////////////////////////////////////////////////////////////////
     -->

    


    <!-- http://www.geneontology.org/formats/oboInOwl#hasExactSynonym -->

    <owl:AnnotationProperty rdf:about="http://www.geneontology.org/formats/oboInOwl#hasExactSynonym"/>
    


    <!-- http://www.geneontology.org/formats/oboInOwl#hasRelatedSynonym -->

    <owl:AnnotationProperty rdf:about="http://www.geneontology.org/formats/oboInOwl#hasRelatedSynonym"/>
    


    <!-- http://www.w3.org/2000/01/rdf-schema#comment -->

    <owl:AnnotationProperty rdf:about="http://www.w3.org/2000/01/rdf-schema#comment"/>
    


    <!-- http://www.w3.org/2000/01/rdf-schema#label -->

    <owl:AnnotationProperty rdf:about="http://www.w3.org/2000/01/rdf-schema#label"/>
    


    <!-- 
    ///////////////////////////////////////////////////////////////////////////////////////
    //
    // Classes
    //
    ///////////////////////////////////////////////////////////////////////////////////////
     -->

    


    <!-- http://purl.obolibrary.org/obo/UO_0000000 -->

    <owl:Class rdf:about="http://purl.obolibrary.org/obo/UO_0000000">
        <rdfs:subClassOf rdf:resource="http://www.w3.org/2002/07/owl#Thing"/>
        <rdfs:comment>&quot;A unit of measurement is a standardized quantity of a physical quality.&quot; [Wikipedia:Wikipedia]</rdfs:comment>
        <rdfs:label>unit</rdfs:label>
    </owl:Class>
    


    <!-- http://purl.obolibrary.org/obo/UO_0000001 -->

    <owl:Class rdf:about="http://purl.obolibrary.org/obo/UO_0000001">
        <rdfs:subClassOf rdf:resource="http://purl.obolibrary.org/obo/UO_0000000"/>
        <rdfs:comment>&quot;A unit which is a standard measure of the distance between two points.&quot; [Wikipedia:Wikipedia]</rdfs:comment>
        <rdfs:label>length unit</rdfs:label>
    </owl:Class>
    


    <!-- http://purl.obolibrary.org/obo/UO_0000002 -->

    <owl:Class rdf:about="http://purl.obolibrary.org/obo/UO_0000002">
        <rdfs:subClassOf rdf:resource="http://purl.obolibrary.org/obo/UO_0000000"/>
        <rdfs:comment>&quot;A unit which is a standard measure of the amount of matter/energy of a physical object.&quot; [Wikipedia:Wikipedia]</rdfs:comment>
        <rdfs:label>mass unit</rdfs:label>
    </owl:Class>
    


    <!-- http://purl.obolibrary.org/obo/UO_0000003 -->

    <owl:Class rdf:about="http://purl.obolibrary.org/obo/UO_0000003">
        <rdfs:subClassOf rdf:resource="http://purl.obolibrary.org/obo/UO_0000000"/>
        <oboInOwl:hasExactSynonym>time derived unit</oboInOwl:hasExactSynonym>
        <rdfs:comment>&quot;A unit which is a standard measure of the dimension in which events occur in sequence.&quot; [Wikipedia:Wikipedia]</rdfs:comment>
        <rdfs:label>time unit</rdfs:label>
    </owl:Class>
    


    <!-- http://purl.obolibrary.org/obo/UO_0000004 -->

    <owl:Class rdf:about="http://purl.obolibrary.org/obo/UO_0000004">
        <rdfs:subClassOf rdf:resource="http://purl.obolibrary.org/obo/UO_0000000"/>
        <rdfs:comment>&quot;A unit which is a standard measure of the flow of electric charge.&quot; [Wikipedia:Wikipedia]</rdfs:comment>
        <rdfs:label>electric current unit</rdfs:label>
    </owl:Class>
    


    <!-- http://purl.obolibrary.org/obo/UO_0000005 -->

    <owl:Class rdf:about="http://purl.obolibrary.org/obo/UO_0000005">
        <rdfs:subClassOf rdf:resource="http://purl.obolibrary.org/obo/UO_0000000"/>
        <oboInOwl:hasExactSynonym>temperature derived unit</oboInOwl:hasExactSynonym>
        <rdfs:comment>&quot;A unit which is a standard measure of the average kinetic energy of the particles in a sample of matter.&quot; [Wikipedia:Wikipedia]</rdfs:comment>
        <rdfs:label>temperature unit</rdfs:label>
    </owl:Class>
    


    <!-- http://purl.obolibrary.org/obo/UO_0000007 -->

    <owl:Class rdf:about="http://purl.obolibrary.org/obo/UO_0000007">
        <rdfs:subClassOf rdf:resource="http://purl.obolibrary.org/obo/UO_0000157"/>
        <rdfs:comment>&quot;A unit which is a standard measure of the wavelength-weighted power emitted by a light source in a particular direction.&quot; [Wikipedia:Wikipedia]</rdfs:comment>
        <rdfs:label>luminous intensity unit</rdfs:label>
    </owl:Class>
    


    <!-- http://purl.obolibrary.org/obo/UO_0000008 -->

    <owl:Class rdf:about="http://purl.obolibrary.org/obo/UO_0000008">
        <rdfs:subClassOf rdf:resource="http://purl.obolibrary.org/obo/UO_0000045"/>
        <rdfs:subClassOf rdf:resource="http://purl.obolibrary.org/obo/UO_1000008"/>
        <oboInOwl:hasExactSynonym>m</oboInOwl:hasExactSynonym>
        <oboInOwl:hasExactSynonym>metre</oboInOwl:hasExactSynonym>
        <rdfs:comment>&quot;A length unit which is equal to the length of the path traveled by light in vacuum during a time interval of 1/299 792 458 of a second.&quot; [BIPM:BIPM, NIST:NIST]</rdfs:comment>
        <rdfs:label>meter</rdfs:label>
    </owl:Class>
    


    <!-- http://purl.obolibrary.org/obo/UO_0000009 -->

    <owl:Class rdf:about="http://purl.obolibrary.org/obo/UO_0000009">
        <rdfs:subClassOf rdf:resource="http://purl.obolibrary.org/obo/UO_0000045"/>
        <rdfs:subClassOf rdf:resource="http://purl.obolibrary.org/obo/UO_1000021"/>
        <oboInOwl:hasExactSynonym>kg</oboInOwl:hasExactSynonym>
        <rdfs:comment>&quot;A mass unit which is equal to the mass of the International Prototype Kilogram kept by the BIPM at Svres, France.&quot; [BIPM:BIPM, NIST:NIST]</rdfs:comment>
        <rdfs:label>kilogram</rdfs:label>
    </owl:Class>
    


    <!-- http://purl.obolibrary.org/obo/UO_0000010 -->

    <owl:Class rdf:about="http://purl.obolibrary.org/obo/UO_0000010">
        <rdfs:subClassOf rdf:resource="http://purl.obolibrary.org/obo/UO_0000045"/>
        <rdfs:subClassOf rdf:resource="http://purl.obolibrary.org/obo/UO_1000010"/>
        <oboInOwl:hasExactSynonym>s</oboInOwl:hasExactSynonym>
        <rdfs:comment>&quot;A time unit which is equal to the duration of 9 192 631 770 periods of the radiation corresponding to the transition between the two hyperfine levels of the ground state of the caesium 133 atom.&quot; [BIPM:BIPM, NIST:NIST]</rdfs:comment>
        <rdfs:label>second</rdfs:label>
    </owl:Class>
    


    <!-- http://purl.obolibrary.org/obo/UO_0000011 -->

    <owl:Class rdf:about="http://purl.obolibrary.org/obo/UO_0000011">
        <rdfs:subClassOf rdf:resource="http://purl.obolibrary.org/obo/UO_0000045"/>
        <rdfs:subClassOf rdf:resource="http://purl.obolibrary.org/obo/UO_1000011"/>
        <oboInOwl:hasExactSynonym>A</oboInOwl:hasExactSynonym>
        <rdfs:comment>&quot;An electric current unit which is equal to the constant current which, if maintained in two straight parallel conductors of infinite length, of negligible circular cross-section, and placed 1 m apart in vacuum, would produce between these conductors a force equal to 2 x 10^[-7] newton per meter of length.&quot; [BIPM:BIPM, NIST:NIST]</rdfs:comment>
        <rdfs:label>ampere</rdfs:label>
    </owl:Class>
    


    <!-- http://purl.obolibrary.org/obo/UO_0000012 -->

    <owl:Class rdf:about="http://purl.obolibrary.org/obo/UO_0000012">
        <rdfs:subClassOf rdf:resource="http://purl.obolibrary.org/obo/UO_0000045"/>
        <rdfs:subClassOf rdf:resource="http://purl.obolibrary.org/obo/UO_1000012"/>
        <oboInOwl:hasExactSynonym>K</oboInOwl:hasExactSynonym>
        <rdfs:comment>&quot;A thermodynamic temperature unit which is equal to the fraction 1/273.16 of the thermodynamic temperature of the triple point of water.&quot; [BIPM:BIPM, NIST:NIST]</rdfs:comment>
        <rdfs:label>kelvin</rdfs:label>
    </owl:Class>
    


    <!-- http://purl.obolibrary.org/obo/UO_0000014 -->

    <owl:Class rdf:about="http://purl.obolibrary.org/obo/UO_0000014">
        <rdfs:subClassOf rdf:resource="http://purl.obolibrary.org/obo/UO_0000045"/>
        <rdfs:subClassOf rdf:resource="http://purl.obolibrary.org/obo/UO_1000014"/>
        <oboInOwl:hasExactSynonym>cd</oboInOwl:hasExactSynonym>
        <rdfs:comment>&quot;A luminous intensity unit which equal to the luminous intensity, in a given direction, of a source that emits monochromatic radiation of frequency 540 x 1012 hertz and that has a radiant intensity in that direction of 1/683 watt per steradian.&quot; [BIPM:BIPM, NIST:NIST]</rdfs:comment>
        <rdfs:label>candela</rdfs:label>
    </owl:Class>
    


    <!-- http://purl.obolibrary.org/obo/UO_0000016 -->

    <owl:Class rdf:about="http://purl.obolibrary.org/obo/UO_0000016">
        <rdfs:subClassOf rdf:resource="http://purl.obolibrary.org/obo/UO_1000008"/>
        <oboInOwl:hasExactSynonym>millimetre</oboInOwl:hasExactSynonym>
        <oboInOwl:hasExactSynonym>mm</oboInOwl:hasExactSynonym>
        <rdfs:comment>&quot;A length unit which is equal to one thousandth of a meter or 10^[-3] m.&quot; [NIST:NIST]</rdfs:comment>
        <rdfs:label>millimeter</rdfs:label>
    </owl:Class>
    


    <!-- http://purl.obolibrary.org/obo/UO_0000021 -->

    <owl:Class rdf:about="http://purl.obolibrary.org/obo/UO_0000021">
        <rdfs:subClassOf rdf:resource="http://purl.obolibrary.org/obo/UO_1000021"/>
        <oboInOwl:hasExactSynonym>g</oboInOwl:hasExactSynonym>
        <rdfs:comment>&quot;A mass unit which is equal to one thousandth of a kilogram or 10^[-3] kg.&quot; [NIST:NIST]</rdfs:comment>
        <rdfs:label>gram</rdfs:label>
    </owl:Class>
    


    <!-- http://purl.obolibrary.org/obo/UO_0000027 -->

    <owl:Class rdf:about="http://purl.obolibrary.org/obo/UO_0000027">
        <rdfs:subClassOf rdf:resource="http://purl.obolibrary.org/obo/UO_1000027"/>
        <oboInOwl:hasExactSynonym>C</oboInOwl:hasExactSynonym>
        <rdfs:comment>&quot;A temperature unit which is equal to one kelvin degree. However, they have their zeros at different points. The centigrade scale has its zero at 273.15 K.&quot; [NIST:NIST]</rdfs:comment>
        <rdfs:label>degree Celsius</rdfs:label>
    </owl:Class>
    


    <!-- http://purl.obolibrary.org/obo/UO_0000031 -->

    <owl:Class rdf:about="http://purl.obolibrary.org/obo/UO_0000031">
        <rdfs:subClassOf rdf:resource="http://purl.obolibrary.org/obo/UO_1000031"/>
        <oboInOwl:hasExactSynonym>min</oboInOwl:hasExactSynonym>
        <rdfs:comment>&quot;A time unit which is equal to 60 seconds.&quot; [Wikipedia:Wikipedia]</rdfs:comment>
        <rdfs:label>minute</rdfs:label>
    </owl:Class>
    


    <!-- http://purl.obolibrary.org/obo/UO_0000032 -->

    <owl:Class rdf:about="http://purl.obolibrary.org/obo/UO_0000032">
        <rdfs:subClassOf rdf:resource="http://purl.obolibrary.org/obo/UO_1000032"/>
        <oboInOwl:hasExactSynonym>h</oboInOwl:hasExactSynonym>
        <rdfs:comment>&quot;A time unit which is equal to 3600 seconds or 60 minutes.&quot; [Wikipedia:Wikipedia]</rdfs:comment>
        <rdfs:label>hour</rdfs:label>
    </owl:Class>
    


    <!-- http://purl.obolibrary.org/obo/UO_0000033 -->

    <owl:Class rdf:about="http://purl.obolibrary.org/obo/UO_0000033">
        <rdfs:subClassOf rdf:resource="http://purl.obolibrary.org/obo/UO_1000033"/>
        <rdfs:comment>&quot;A time unit which is equal to 24 hours.&quot; [Wikipedia:Wikipedia]</rdfs:comment>
        <rdfs:label>day</rdfs:label>
    </owl:Class>
    


    <!-- http://purl.obolibrary.org/obo/UO_0000034 -->

    <owl:Class rdf:about="http://purl.obolibrary.org/obo/UO_0000034">
        <rdfs:subClassOf rdf:resource="http://purl.obolibrary.org/obo/UO_1000034"/>
        <rdfs:comment>&quot;A time unit which is equal to 7 days.&quot; [Wikipedia:Wikipedia]</rdfs:comment>
        <rdfs:label>week</rdfs:label>
    </owl:Class>
    


    <!-- http://purl.obolibrary.org/obo/UO_0000035 -->

    <owl:Class rdf:about="http://purl.obolibrary.org/obo/UO_0000035">
        <rdfs:subClassOf rdf:resource="http://purl.obolibrary.org/obo/UO_1000035"/>
        <rdfs:comment>&quot;A time unit which is approximately equal to the length of time of one of cycle of the moon&apos;s phases which in science is taken to be equal to 30 days.&quot; [Wikipedia:Wikipedia]</rdfs:comment>
        <rdfs:label>month</rdfs:label>
    </owl:Class>
    


    <!-- http://purl.obolibrary.org/obo/UO_0000036 -->

    <owl:Class rdf:about="http://purl.obolibrary.org/obo/UO_0000036">
        <rdfs:subClassOf rdf:resource="http://purl.obolibrary.org/obo/UO_1000036"/>
        <rdfs:comment>&quot;A time unit which is equal to 12 months which in science is taken to be equal to 365.25 days.&quot; [Wikipedia:Wikipedia]</rdfs:comment>
        <rdfs:label>year</rdfs:label>
    </owl:Class>
    


    <!-- http://purl.obolibrary.org/obo/UO_0000045 -->

    <owl:Class rdf:about="http://purl.obolibrary.org/obo/UO_0000045">
        <rdfs:subClassOf rdf:resource="http://purl.obolibrary.org/obo/UO_0000000"/>
        <rdfs:comment>&quot;A unit which is one of a particular measure to which all measures of that type can be related.&quot; [NIST:NIST]</rdfs:comment>
        <rdfs:label>base unit</rdfs:label>
    </owl:Class>
    


    <!-- http://purl.obolibrary.org/obo/UO_0000046 -->

    <owl:Class rdf:about="http://purl.obolibrary.org/obo/UO_0000046">
        <rdfs:subClassOf rdf:resource="http://www.w3.org/2002/07/owl#Thing"/>
        <rdfs:label>prefix</rdfs:label>
    </owl:Class>
    


    <!-- http://purl.obolibrary.org/obo/UO_0000047 -->

    <owl:Class rdf:about="http://purl.obolibrary.org/obo/UO_0000047">
        <rdfs:subClassOf rdf:resource="http://purl.obolibrary.org/obo/UO_0000000"/>
        <rdfs:comment>&quot;A unit which is a standard measure of the amount of a 2-dimensional flat surface.&quot; [UOC:GVG]</rdfs:comment>
        <rdfs:label>area unit</rdfs:label>
    </owl:Class>
    


    <!-- http://purl.obolibrary.org/obo/UO_0000051 -->

    <owl:Class rdf:about="http://purl.obolibrary.org/obo/UO_0000051">
        <rdfs:subClassOf rdf:resource="http://purl.obolibrary.org/obo/UO_0000000"/>
        <rdfs:comment>&quot;A unit which represents a standard measurement of how much of a given substance there is mixed with another substance.&quot; [UOC:GVG]</rdfs:comment>
        <rdfs:label>concentration unit</rdfs:label>
    </owl:Class>
    


    <!-- http://purl.obolibrary.org/obo/UO_0000052 -->

    <owl:Class rdf:about="http://purl.obolibrary.org/obo/UO_0000052">
        <rdfs:subClassOf rdf:resource="http://purl.obolibrary.org/obo/UO_0000182"/>
        <oboInOwl:hasExactSynonym>mass per unit volume</oboInOwl:hasExactSynonym>
        <rdfs:comment>&quot;A density unit which is a standard measure of the mass of a substance in a given volume.&quot; [UOC:GVG]</rdfs:comment>
        <rdfs:label>mass density unit</rdfs:label>
    </owl:Class>
    


    <!-- http://purl.obolibrary.org/obo/UO_0000054 -->

    <owl:Class rdf:about="http://purl.obolibrary.org/obo/UO_0000054">
        <rdfs:subClassOf rdf:resource="http://purl.obolibrary.org/obo/UO_0000182"/>
        <oboInOwl:hasExactSynonym>mass per unit area unit</oboInOwl:hasExactSynonym>
        <rdfs:comment>&quot;A density unit which is a standard measure of the mass exerting an influence on a given area.&quot; [Wikipedia:Wikipedia]</rdfs:comment>
        <rdfs:label>area density unit</rdfs:label>
    </owl:Class>
    


    <!-- http://purl.obolibrary.org/obo/UO_0000058 -->

    <owl:Class rdf:about="http://purl.obolibrary.org/obo/UO_0000058">
        <rdfs:subClassOf rdf:resource="http://purl.obolibrary.org/obo/UO_0000105"/>
        <rdfs:comment>&quot;A unit which is a standard measure of the number of rotations in a given time.&quot; [NIST:NIST]</rdfs:comment>
        <rdfs:label>rotational frequency unit</rdfs:label>
    </owl:Class>
    


    <!-- http://purl.obolibrary.org/obo/UO_0000060 -->

    <owl:Class rdf:about="http://purl.obolibrary.org/obo/UO_0000060">
        <rdfs:subClassOf rdf:resource="http://purl.obolibrary.org/obo/UO_0000000"/>
        <rdfs:comment>&quot;A unit which is a standard measure of the rate of movement. Speed is measured in the same physical units of measurement as velocity, but does not contain the element of direction that velocity has. Speed is thus the magnitude component of velocity.&quot; [Wikipedia:Wikipedia]</rdfs:comment>
        <rdfs:label>speed/velocity unit</rdfs:label>
    </owl:Class>
    


    <!-- http://purl.obolibrary.org/obo/UO_0000080 -->

    <owl:Class rdf:about="http://purl.obolibrary.org/obo/UO_0000080">
        <rdfs:subClassOf rdf:resource="http://purl.obolibrary.org/obo/UO_1000080"/>
        <oboInOwl:hasExactSynonym>m^[2]</oboInOwl:hasExactSynonym>
        <oboInOwl:hasExactSynonym>square metre</oboInOwl:hasExactSynonym>
        <rdfs:comment>&quot;An area unit which is equal to an area enclosed by a square with sides each 1 meter long.&quot; [NIST:NIST]</rdfs:comment>
        <rdfs:label>square meter</rdfs:label>
    </owl:Class>
    


    <!-- http://purl.obolibrary.org/obo/UO_0000082 -->

    <owl:Class rdf:about="http://purl.obolibrary.org/obo/UO_0000082">
        <rdfs:subClassOf rdf:resource="http://purl.obolibrary.org/obo/UO_1000082"/>
        <oboInOwl:hasExactSynonym>mm^[2]</oboInOwl:hasExactSynonym>
        <oboInOwl:hasExactSynonym>square millimetre</oboInOwl:hasExactSynonym>
        <rdfs:comment>&quot;An area unit which is equal to one millionth of a square meter or 10^[-6] m^[2].&quot; [NIST:NIST]</rdfs:comment>
        <rdfs:label>square millimeter</rdfs:label>
    </owl:Class>
    


    <!-- http://purl.obolibrary.org/obo/UO_0000083 -->

    <owl:Class rdf:about="http://purl.obolibrary.org/obo/UO_0000083">
        <rdfs:subClassOf rdf:resource="http://purl.obolibrary.org/obo/UO_0000052"/>
        <oboInOwl:hasExactSynonym>kg/m^[3]</oboInOwl:hasExactSynonym>
        <oboInOwl:hasExactSynonym>kilogram per cubic metre</oboInOwl:hasExactSynonym>
        <rdfs:comment>&quot;A mass unit density which is equal to mass of an object in kilograms divided by the volume in cubic meters.&quot; [UOC:GVG]</rdfs:comment>
        <rdfs:label>kilogram per cubic meter</rdfs:label>
    </owl:Class>
    


    <!-- http://purl.obolibrary.org/obo/UO_0000086 -->

    <owl:Class rdf:about="http://purl.obolibrary.org/obo/UO_0000086">
        <rdfs:subClassOf rdf:resource="http://purl.obolibrary.org/obo/UO_1010049"/>
        <oboInOwl:hasExactSynonym>kg/m^[2]</oboInOwl:hasExactSynonym>
        <oboInOwl:hasExactSynonym>kilogram per square metre</oboInOwl:hasExactSynonym>
        <rdfs:comment>&quot;An area density unit which is equal to the mass of an object in kilograms divided by the surface area in meters squared.&quot; [NIST:NIST]</rdfs:comment>
        <rdfs:label>kilogram per square meter</rdfs:label>
    </owl:Class>
    


    <!-- http://purl.obolibrary.org/obo/UO_0000092 -->

    <owl:Class rdf:about="http://purl.obolibrary.org/obo/UO_0000092">
        <rdfs:subClassOf rdf:resource="http://purl.obolibrary.org/obo/UO_1000092"/>
        <oboInOwl:hasExactSynonym>1/s</oboInOwl:hasExactSynonym>
        <oboInOwl:hasExactSynonym>one turn per second</oboInOwl:hasExactSynonym>
        <rdfs:comment>&quot;A rotational frequency unit which is equal to the number complete turn in a period of time that equals to 1 second.&quot; [NIST:NIST]</rdfs:comment>
        <rdfs:label>turns per second</rdfs:label>
    </owl:Class>
    


    <!-- http://purl.obolibrary.org/obo/UO_0000094 -->

    <owl:Class rdf:about="http://purl.obolibrary.org/obo/UO_0000094">
        <rdfs:subClassOf rdf:resource="http://purl.obolibrary.org/obo/UO_1000094"/>
        <oboInOwl:hasExactSynonym>m/s</oboInOwl:hasExactSynonym>
        <oboInOwl:hasExactSynonym>metre per second</oboInOwl:hasExactSynonym>
        <rdfs:comment>&quot;A speed/velocity unit which is equal to the speed of an object traveling 1 meter distance in one second.&quot; [NIST:NIST]</rdfs:comment>
        <rdfs:label>meter per second</rdfs:label>
    </owl:Class>
    


    <!-- http://purl.obolibrary.org/obo/UO_0000095 -->

    <owl:Class rdf:about="http://purl.obolibrary.org/obo/UO_0000095">
        <rdfs:subClassOf rdf:resource="http://purl.obolibrary.org/obo/UO_0000000"/>
        <rdfs:comment>&quot;A unit which is a standard measure of the amount of space occupied by any substance, whether solid, liquid, or gas.&quot; [NIST:NIST]</rdfs:comment>
        <rdfs:label>volume unit</rdfs:label>
    </owl:Class>
    


    <!-- http://purl.obolibrary.org/obo/UO_0000096 -->

    <owl:Class rdf:about="http://purl.obolibrary.org/obo/UO_0000096">
        <rdfs:subClassOf rdf:resource="http://purl.obolibrary.org/obo/UO_1000096"/>
        <oboInOwl:hasExactSynonym>cubic metre</oboInOwl:hasExactSynonym>
        <oboInOwl:hasExactSynonym>m^[3]</oboInOwl:hasExactSynonym>
        <rdfs:comment>&quot;A volume unit which is equal to the volume of a cube with edges one meter in length. One cubic meter equals to 1000 liters.&quot; [NIST:NIST]</rdfs:comment>
        <rdfs:label>cubic meter</rdfs:label>
    </owl:Class>
    


    <!-- http://purl.obolibrary.org/obo/UO_0000097 -->

    <owl:Class rdf:about="http://purl.obolibrary.org/obo/UO_0000097">
        <rdfs:subClassOf rdf:resource="http://purl.obolibrary.org/obo/UO_1000097"/>
        <oboInOwl:hasExactSynonym>cc</oboInOwl:hasExactSynonym>
        <oboInOwl:hasExactSynonym>cm^3</oboInOwl:hasExactSynonym>
        <oboInOwl:hasExactSynonym>cubic centimetre</oboInOwl:hasExactSynonym>
        <rdfs:comment>&quot;A volume unit which is equal to one millionth of a cubic meter or 10^[-9] m^[3], or to 1 ml.&quot; [NIST:NIST]</rdfs:comment>
        <rdfs:label>cubic centimeter</rdfs:label>
    </owl:Class>
    


    <!-- http://purl.obolibrary.org/obo/UO_0000099 -->

    <owl:Class rdf:about="http://purl.obolibrary.org/obo/UO_0000099">
        <rdfs:subClassOf rdf:resource="http://purl.obolibrary.org/obo/UO_1000099"/>
        <oboInOwl:hasExactSynonym>L</oboInOwl:hasExactSynonym>
        <oboInOwl:hasExactSynonym>l</oboInOwl:hasExactSynonym>
        <oboInOwl:hasExactSynonym>litre</oboInOwl:hasExactSynonym>
        <rdfs:comment>&quot;A volume unit which is equal to one thousandth of a cubic meter or 10^[-3] m^[3], or to 1 decimeter.&quot; [NIST:NIST]</rdfs:comment>
        <rdfs:label>liter</rdfs:label>
    </owl:Class>
    


    <!-- http://purl.obolibrary.org/obo/UO_0000105 -->

    <owl:Class rdf:about="http://purl.obolibrary.org/obo/UO_0000105">
        <rdfs:subClassOf rdf:resource="http://purl.obolibrary.org/obo/UO_0000000"/>
        <rdfs:comment>&quot;A unit which is a standard measure of the number of repetitive actions in a particular time.&quot; [NIST:NIST]</rdfs:comment>
        <rdfs:label>frequency unit</rdfs:label>
    </owl:Class>
    


    <!-- http://purl.obolibrary.org/obo/UO_0000106 -->

    <owl:Class rdf:about="http://purl.obolibrary.org/obo/UO_0000106">
        <rdfs:subClassOf rdf:resource="http://purl.obolibrary.org/obo/UO_1000106"/>
        <oboInOwl:hasExactSynonym>Hz</oboInOwl:hasExactSynonym>
        <oboInOwl:hasExactSynonym>s^1</oboInOwl:hasExactSynonym>
        <rdfs:comment>&quot;A frequency unit which is equal to 1 complete cycle of a recurring phenomenon in 1 second.&quot; [NIST:NIST]</rdfs:comment>
        <rdfs:label>hertz</rdfs:label>
    </owl:Class>
    


    <!-- http://purl.obolibrary.org/obo/UO_0000107 -->

    <owl:Class rdf:about="http://purl.obolibrary.org/obo/UO_0000107">
        <rdfs:subClassOf rdf:resource="http://purl.obolibrary.org/obo/UO_0000000"/>
        <rdfs:comment>&quot;A unit which is a standard measure of the force is applied when a mass is accelerated.&quot; [NIST:NIST]</rdfs:comment>
        <rdfs:label>force unit</rdfs:label>
    </owl:Class>
    


    <!-- http://purl.obolibrary.org/obo/UO_0000108 -->

    <owl:Class rdf:about="http://purl.obolibrary.org/obo/UO_0000108">
        <rdfs:subClassOf rdf:resource="http://purl.obolibrary.org/obo/UO_1000108"/>
        <oboInOwl:hasExactSynonym>N</oboInOwl:hasExactSynonym>
        <rdfs:comment>&quot;A force unit which is equal to the force required to cause an acceleration of 1m/s2 of a mass of 1 Kg in the direction of the force.&quot; [NIST:NIST]</rdfs:comment>
        <rdfs:label>newton</rdfs:label>
    </owl:Class>
    


    <!-- http://purl.obolibrary.org/obo/UO_0000109 -->

    <owl:Class rdf:about="http://purl.obolibrary.org/obo/UO_0000109">
        <rdfs:subClassOf rdf:resource="http://purl.obolibrary.org/obo/UO_0000000"/>
        <rdfs:comment>&quot;A unit which is a standard measure of the force applied to a given area.&quot; [NIST:NIST]</rdfs:comment>
        <rdfs:label>pressure unit</rdfs:label>
    </owl:Class>
    


    <!-- http://purl.obolibrary.org/obo/UO_0000110 -->

    <owl:Class rdf:about="http://purl.obolibrary.org/obo/UO_0000110">
        <rdfs:subClassOf rdf:resource="http://purl.obolibrary.org/obo/UO_1000110"/>
        <oboInOwl:hasExactSynonym>Pa</oboInOwl:hasExactSynonym>
        <rdfs:comment>&quot;A pressure unit which is equal to the pressure or stress on a surface caused by a force of 1 newton spread over a surface of 1 m^[2].&quot; [NIST:NIST]</rdfs:comment>
        <rdfs:label>pascal</rdfs:label>
    </owl:Class>
    


    <!-- http://purl.obolibrary.org/obo/UO_0000111 -->

    <owl:Class rdf:about="http://purl.obolibrary.org/obo/UO_0000111">
        <rdfs:subClassOf rdf:resource="http://purl.obolibrary.org/obo/UO_0000000"/>
        <rdfs:comment>&quot;A unit which is a standard measure of the work done by a certain force (gravitational, electric, magnetic, force of inertia, etc).&quot; [NIST:NIST]</rdfs:comment>
        <rdfs:label>energy unit</rdfs:label>
    </owl:Class>
    


    <!-- http://purl.obolibrary.org/obo/UO_0000112 -->

    <owl:Class rdf:about="http://purl.obolibrary.org/obo/UO_0000112">
        <rdfs:subClassOf rdf:resource="http://purl.obolibrary.org/obo/UO_1000112"/>
        <oboInOwl:hasExactSynonym>J</oboInOwl:hasExactSynonym>
        <rdfs:comment>&quot;An energy unit which is equal to the energy required when a force of 1 newton moves an object 1 meter in the direction of the force.&quot; [NIST:NIST]</rdfs:comment>
        <rdfs:label>joule</rdfs:label>
    </owl:Class>
    


    <!-- http://purl.obolibrary.org/obo/UO_0000113 -->

    <owl:Class rdf:about="http://purl.obolibrary.org/obo/UO_0000113">
        <rdfs:subClassOf rdf:resource="http://purl.obolibrary.org/obo/UO_0000000"/>
        <rdfs:comment>&quot;A unit which is a standard measure power or the rate of doing work.&quot; [NIST:NIST]</rdfs:comment>
        <rdfs:label>power unit</rdfs:label>
    </owl:Class>
    


    <!-- http://purl.obolibrary.org/obo/UO_0000114 -->

    <owl:Class rdf:about="http://purl.obolibrary.org/obo/UO_0000114">
        <rdfs:subClassOf rdf:resource="http://purl.obolibrary.org/obo/UO_1000114"/>
        <oboInOwl:hasExactSynonym>W</oboInOwl:hasExactSynonym>
        <rdfs:comment>&quot;A power unit which is equal to the power used when work is done at the rate of 1 joule per second.&quot; [NIST:NIST]</rdfs:comment>
        <rdfs:label>watt</rdfs:label>
    </owl:Class>
    


    <!-- http://purl.obolibrary.org/obo/UO_0000115 -->

    <owl:Class rdf:about="http://purl.obolibrary.org/obo/UO_0000115">
        <rdfs:subClassOf rdf:resource="http://purl.obolibrary.org/obo/UO_0000157"/>
        <rdfs:comment>&quot;A unit which is a standard measure of the luminous flux incident on a unit area.&quot; [Wikipedia:Wikipedia]</rdfs:comment>
        <rdfs:label>illuminance unit</rdfs:label>
    </owl:Class>
    


    <!-- http://purl.obolibrary.org/obo/UO_0000116 -->

    <owl:Class rdf:about="http://purl.obolibrary.org/obo/UO_0000116">
        <rdfs:subClassOf rdf:resource="http://purl.obolibrary.org/obo/UO_1000116"/>
        <oboInOwl:hasExactSynonym>lx</oboInOwl:hasExactSynonym>
        <rdfs:comment>&quot;An illuminance unit which is equal to the illuminance produced by 1 lumen evenly spread over an area 1 m^[2].&quot; [NIST:NIST]</rdfs:comment>
        <rdfs:label>lux</rdfs:label>
    </owl:Class>
    


    <!-- http://purl.obolibrary.org/obo/UO_0000117 -->

    <owl:Class rdf:about="http://purl.obolibrary.org/obo/UO_0000117">
        <rdfs:subClassOf rdf:resource="http://purl.obolibrary.org/obo/UO_0000157"/>
        <rdfs:comment>&quot;A unit which is a standard measure of the flow of radiant energy.&quot; [Wikipedia:Wikipedia]</rdfs:comment>
        <rdfs:label>luminous flux unit</rdfs:label>
    </owl:Class>
    


    <!-- http://purl.obolibrary.org/obo/UO_0000118 -->

    <owl:Class rdf:about="http://purl.obolibrary.org/obo/UO_0000118">
        <rdfs:subClassOf rdf:resource="http://purl.obolibrary.org/obo/UO_1000118"/>
        <oboInOwl:hasExactSynonym>lm</oboInOwl:hasExactSynonym>
        <rdfs:comment>&quot;A luminous flux unit which is equal to the luminous flux emitted into 1 steradian by a point source of 1 candela.&quot; [NIST:NIST]</rdfs:comment>
        <rdfs:label>lumen</rdfs:label>
    </owl:Class>
    


    <!-- http://purl.obolibrary.org/obo/UO_0000121 -->

    <owl:Class rdf:about="http://purl.obolibrary.org/obo/UO_0000121">
        <rdfs:subClassOf rdf:resource="http://purl.obolibrary.org/obo/UO_0000000"/>
        <rdfs:comment>&quot;A unit which is a standard measure of the figure or space formed by the junction of two lines or planes.&quot; [Wikipedia:Wikipedia]</rdfs:comment>
        <rdfs:label>angle unit</rdfs:label>
    </owl:Class>
    


    <!-- http://purl.obolibrary.org/obo/UO_0000122 -->

    <owl:Class rdf:about="http://purl.obolibrary.org/obo/UO_0000122">
        <rdfs:subClassOf rdf:resource="http://purl.obolibrary.org/obo/UO_0000121"/>
        <rdfs:comment>&quot;A unit which is a standard measure of the angle formed by two straight lines in the same plane.&quot; [Wikipedia:Wikipedia]</rdfs:comment>
        <rdfs:label>plane angle unit</rdfs:label>
    </owl:Class>
    


    <!-- http://purl.obolibrary.org/obo/UO_0000123 -->

    <owl:Class rdf:about="http://purl.obolibrary.org/obo/UO_0000123">
        <rdfs:subClassOf rdf:resource="http://purl.obolibrary.org/obo/UO_1000123"/>
        <oboInOwl:hasExactSynonym>rad</oboInOwl:hasExactSynonym>
        <rdfs:comment>&quot;A plane angle unit which is equal to the angle subtended at the center of a circle by an arc equal in length to the radius of the circle, approximately 57 degrees 17 minutes and 44.6 seconds.&quot; [NIST:NIST]</rdfs:comment>
        <rdfs:label>radian</rdfs:label>
    </owl:Class>
    


    <!-- http://purl.obolibrary.org/obo/UO_0000154 -->

    <owl:Class rdf:about="http://purl.obolibrary.org/obo/UO_0000154">
        <rdfs:subClassOf rdf:resource="http://purl.obolibrary.org/obo/UO_0000157"/>
        <rdfs:comment>&quot;A unit which is a standard measure of the power of electromagnetic radiation at a surface, per unit area.&quot; [Wikipedia:Wikipedia]</rdfs:comment>
        <rdfs:label>irradiance unit</rdfs:label>
    </owl:Class>
    


    <!-- http://purl.obolibrary.org/obo/UO_0000155 -->

    <owl:Class rdf:about="http://purl.obolibrary.org/obo/UO_0000155">
        <rdfs:subClassOf rdf:resource="http://purl.obolibrary.org/obo/UO_1000155"/>
        <oboInOwl:hasExactSynonym>W/m^[2]</oboInOwl:hasExactSynonym>
        <oboInOwl:hasExactSynonym>watt per square metre</oboInOwl:hasExactSynonym>
        <rdfs:comment>&quot;An irradiance unit which is equal to 1 watt of radiant power incident per one square meter surface area.&quot; [NIST:NIST]</rdfs:comment>
        <rdfs:label>watt per square meter</rdfs:label>
    </owl:Class>
    


    <!-- http://purl.obolibrary.org/obo/UO_0000157 -->

    <owl:Class rdf:about="http://purl.obolibrary.org/obo/UO_0000157">
        <rdfs:subClassOf rdf:resource="http://purl.obolibrary.org/obo/UO_0000000"/>
        <rdfs:comment>&quot;A unit which is a standard measure of the intensity of light.&quot; [NIST:NIST]</rdfs:comment>
        <rdfs:label>light unit</rdfs:label>
    </owl:Class>
    


    <!-- http://purl.obolibrary.org/obo/UO_0000166 -->

    <owl:Class rdf:about="http://purl.obolibrary.org/obo/UO_0000166">
        <rdfs:subClassOf rdf:resource="http://purl.obolibrary.org/obo/UO_0000186"/>
        <rdfs:comment>&quot;A dimensionless concentration notation which describes the amount of one substance in another. It is the ratio of the amount of the substance of interest to the amount of that substance plus the amount of the substance.&quot; [Wikipedia:Wikipedia]</rdfs:comment>
        <rdfs:label>parts per notation unit</rdfs:label>
    </owl:Class>
    


    <!-- http://purl.obolibrary.org/obo/UO_0000169 -->

    <owl:Class rdf:about="http://purl.obolibrary.org/obo/UO_0000169">
        <rdfs:subClassOf rdf:resource="http://purl.obolibrary.org/obo/UO_1000169"/>
        <oboInOwl:hasExactSynonym>10^[-6]</oboInOwl:hasExactSynonym>
        <oboInOwl:hasExactSynonym>ppm</oboInOwl:hasExactSynonym>
        <rdfs:comment>&quot;A dimensionless concentration notation which denotes the amount of a given substance in a total amount of 1,000,000 regardless of the units of measure used as long as they are the same or 1 part in 10^[6].&quot; [UOC:GVG]</rdfs:comment>
        <rdfs:label>parts per million</rdfs:label>
    </owl:Class>
    


    <!-- http://purl.obolibrary.org/obo/UO_0000182 -->

    <owl:Class rdf:about="http://purl.obolibrary.org/obo/UO_0000182">
        <rdfs:subClassOf rdf:resource="http://purl.obolibrary.org/obo/UO_0000000"/>
        <rdfs:comment>&quot;A unit which is a standard measure of the influence exerted by some mass.&quot; [Wikipedia:Wikipedia]</rdfs:comment>
        <rdfs:label>density unit</rdfs:label>
    </owl:Class>
    


    <!-- http://purl.obolibrary.org/obo/UO_0000185 -->

    <owl:Class rdf:about="http://purl.obolibrary.org/obo/UO_0000185">
        <rdfs:subClassOf rdf:resource="http://purl.obolibrary.org/obo/UO_1000185"/>
        <rdfs:comment>&quot;A plane angle unit which is equal to 1/360 of a full rotation or 1.7453310^[-2] rad.&quot; [Wikipedia:Wikipedia]</rdfs:comment>
        <rdfs:label>degree</rdfs:label>
    </owl:Class>
    


    <!-- http://purl.obolibrary.org/obo/UO_0000186 -->

    <owl:Class rdf:about="http://purl.obolibrary.org/obo/UO_0000186">
        <rdfs:subClassOf rdf:resource="http://purl.obolibrary.org/obo/UO_0000000"/>
        <rdfs:comment>&quot;A unit which is a standard measure of physical quantity consisting of only a numerical number without any units.&quot; [Wikipedia:Wikipedia]</rdfs:comment>
        <rdfs:label>dimensionless unit</rdfs:label>
    </owl:Class>
    


    <!-- http://purl.obolibrary.org/obo/UO_0000187 -->

    <owl:Class rdf:about="http://purl.obolibrary.org/obo/UO_0000187">
        <rdfs:subClassOf rdf:resource="http://purl.obolibrary.org/obo/UO_0000190"/>
        <oboInOwl:hasExactSynonym>%</oboInOwl:hasExactSynonym>
        <rdfs:comment>&quot;A dimensionless ratio unit which denotes numbers as fractions of 100.&quot; [Wikipedia:Wikipedia]</rdfs:comment>
        <rdfs:label>percent</rdfs:label>
    </owl:Class>
    


    <!-- http://purl.obolibrary.org/obo/UO_0000188 -->

    <owl:Class rdf:about="http://purl.obolibrary.org/obo/UO_0000188">
        <rdfs:subClassOf rdf:resource="http://purl.obolibrary.org/obo/UO_1000188"/>
        <rdfs:comment>&quot;A dimensionless unit which denoted an irrational real number, approximately equal to 3.14159 which is the ratio of a circle&apos;s circumference to its diameter in Euclidean geometry.&quot; [Wikipedia:Wikipedia]</rdfs:comment>
        <rdfs:label>pi</rdfs:label>
    </owl:Class>
    


    <!-- http://purl.obolibrary.org/obo/UO_0000190 -->

    <owl:Class rdf:about="http://purl.obolibrary.org/obo/UO_0000190">
        <rdfs:subClassOf rdf:resource="http://purl.obolibrary.org/obo/UO_0000186"/>
        <rdfs:comment>&quot;A dimensionless unit which denotes an amount or magnitude of one quantity relative to another.&quot; [Wikipedia:Wikipedia]</rdfs:comment>
        <rdfs:label>ratio unit</rdfs:label>
    </owl:Class>
    


    <!-- http://purl.obolibrary.org/obo/UO_0000196 -->

    <owl:Class rdf:about="http://purl.obolibrary.org/obo/UO_0000196">
        <rdfs:subClassOf rdf:resource="http://purl.obolibrary.org/obo/UO_1000196"/>
        <rdfs:comment>&quot;A dimensionless concentration notation which denotes the acidity of a solution in terms of activity of hydrogen ions (H+).&quot; [Wikipedia:Wikipedia]</rdfs:comment>
        <rdfs:label>pH</rdfs:label>
    </owl:Class>
    


    <!-- http://purl.obolibrary.org/obo/UO_0000217 -->

    <owl:Class rdf:about="http://purl.obolibrary.org/obo/UO_0000217">
        <rdfs:subClassOf rdf:resource="http://purl.obolibrary.org/obo/UO_0000000"/>
        <rdfs:comment>&quot;A unit which is a standard measure of the work done per unit charge as a charge is moved between two points in an electric field.&quot; [Wikipedia:Wikipedia]</rdfs:comment>
        <rdfs:label>electric potential difference unit</rdfs:label>
    </owl:Class>
    


    <!-- http://purl.obolibrary.org/obo/UO_0000218 -->

    <owl:Class rdf:about="http://purl.obolibrary.org/obo/UO_0000218">
        <rdfs:subClassOf rdf:resource="http://purl.obolibrary.org/obo/UO_1000218"/>
        <oboInOwl:hasExactSynonym>V</oboInOwl:hasExactSynonym>
        <rdfs:comment>&quot;An electric potential difference unit which is equal to the work per unit charge. One volt is the potential difference required to move one coulomb of charge between two points in a circuit while using one joule of energy.&quot; [Wikipedia:Wikipedia]</rdfs:comment>
        <rdfs:label>volt</rdfs:label>
    </owl:Class>
    


    <!-- http://purl.obolibrary.org/obo/UO_0000219 -->

    <owl:Class rdf:about="http://purl.obolibrary.org/obo/UO_0000219">
        <rdfs:subClassOf rdf:resource="http://purl.obolibrary.org/obo/UO_0000000"/>
        <rdfs:comment>&quot;A unit which is a standard measure of the quantity of unbalanced electricity in a body (either positive or negative) and construed as an excess or deficiency of electrons.&quot; [WordNet:WordNet]</rdfs:comment>
        <rdfs:label>electric charge</rdfs:label>
    </owl:Class>
    


    <!-- http://purl.obolibrary.org/obo/UO_0000220 -->

    <owl:Class rdf:about="http://purl.obolibrary.org/obo/UO_0000220">
        <rdfs:subClassOf rdf:resource="http://purl.obolibrary.org/obo/UO_1000220"/>
        <oboInOwl:hasExactSynonym>C</oboInOwl:hasExactSynonym>
        <rdfs:comment>&quot;An electrical charge unit which is equal to the amount of charge transferred by a current of 1 ampere in 1 second.&quot; [WordNet:WordNet]</rdfs:comment>
        <rdfs:label>coulomb</rdfs:label>
    </owl:Class>
    


    <!-- http://purl.obolibrary.org/obo/UO_0000223 -->

    <owl:Class rdf:about="http://purl.obolibrary.org/obo/UO_0000223">
        <rdfs:subClassOf rdf:resource="http://purl.obolibrary.org/obo/UO_1000223"/>
        <oboInOwl:hasExactSynonym>Wh</oboInOwl:hasExactSynonym>
        <rdfs:comment>&quot;An energy unit which is equal to the amount of electrical energy equivalent to a one-watt load drawing power for one hour.&quot; [Wikipedia:Wikipedia]</rdfs:comment>
        <rdfs:label>watt-hour</rdfs:label>
    </owl:Class>
    


    <!-- http://purl.obolibrary.org/obo/UO_0000224 -->

    <owl:Class rdf:about="http://purl.obolibrary.org/obo/UO_0000224">
        <rdfs:subClassOf rdf:resource="http://purl.obolibrary.org/obo/UO_1000223"/>
        <rdfs:comment>&quot;An energy unit which is equal to 1,000 watt-hours.&quot; [Wikipedia:Wikipedia]</rdfs:comment>
        <rdfs:label>kilowatt-hour</rdfs:label>
    </owl:Class>
    


    <!-- http://purl.obolibrary.org/obo/UO_0000231 -->

    <owl:Class rdf:about="http://purl.obolibrary.org/obo/UO_0000231">
        <rdfs:subClassOf rdf:resource="http://purl.obolibrary.org/obo/UO_0000000"/>
        <rdfs:comment>&quot;A unit which is a standard measure of the amount of information.&quot; [Wikipedia:Wikipedia]</rdfs:comment>
        <rdfs:label>information unit</rdfs:label>
    </owl:Class>
    


    <!-- http://purl.obolibrary.org/obo/UO_0000232 -->

    <owl:Class rdf:about="http://purl.obolibrary.org/obo/UO_0000232">
        <rdfs:subClassOf rdf:resource="http://purl.obolibrary.org/obo/UO_1000232"/>
        <rdfs:comment>&quot;An information unit which refers to a digit in the binary numeral system, which consists of base 2 digits (ie there are only 2 possible values: 0 or 1).&quot; [Wikipedia:Wikipedia]</rdfs:comment>
        <rdfs:label>bit</rdfs:label>
    </owl:Class>
    


    <!-- http://purl.obolibrary.org/obo/UO_0000233 -->

    <owl:Class rdf:about="http://purl.obolibrary.org/obo/UO_0000233">
        <rdfs:subClassOf rdf:resource="http://purl.obolibrary.org/obo/UO_1000233"/>
        <oboInOwl:hasExactSynonym>B</oboInOwl:hasExactSynonym>
        <rdfs:comment>&quot;An information unit which is equal to 8 bits.&quot; [Wikipedia:Wikipedia]</rdfs:comment>
        <rdfs:label>byte</rdfs:label>
    </owl:Class>
    


    <!-- http://purl.obolibrary.org/obo/UO_0000234 -->

    <owl:Class rdf:about="http://purl.obolibrary.org/obo/UO_0000234">
        <rdfs:subClassOf rdf:resource="http://purl.obolibrary.org/obo/UO_1000233"/>
        <oboInOwl:hasExactSynonym>kB</oboInOwl:hasExactSynonym>
        <rdfs:comment>&quot;An information unit which is equal to 1000 bytes.&quot; [Wikipedia:Wikipedia]</rdfs:comment>
        <rdfs:label>kilobyte</rdfs:label>
    </owl:Class>
    


    <!-- http://purl.obolibrary.org/obo/UO_0000235 -->

    <owl:Class rdf:about="http://purl.obolibrary.org/obo/UO_0000235">
        <rdfs:subClassOf rdf:resource="http://purl.obolibrary.org/obo/UO_1000233"/>
        <oboInOwl:hasExactSynonym>MB</oboInOwl:hasExactSynonym>
        <rdfs:comment>&quot;An information unit which is equal to 1000 kB.&quot; [Wikipedia:Wikipedia]</rdfs:comment>
        <rdfs:label>megabyte</rdfs:label>
    </owl:Class>
    


    <!-- http://purl.obolibrary.org/obo/UO_0000248 -->

    <owl:Class rdf:about="http://purl.obolibrary.org/obo/UO_0000248">
        <rdfs:subClassOf rdf:resource="http://purl.obolibrary.org/obo/UO_1000218"/>
        <oboInOwl:hasExactSynonym>kV</oboInOwl:hasExactSynonym>
        <rdfs:comment>&quot;An electric potential difference unit which is equal to one thousand volts or 10^[3] V.&quot; [UOC:GVG]</rdfs:comment>
        <rdfs:label>kilovolt</rdfs:label>
    </owl:Class>
    


    <!-- http://purl.obolibrary.org/obo/UO_0000252 -->

    <owl:Class rdf:about="http://purl.obolibrary.org/obo/UO_0000252">
        <rdfs:subClassOf rdf:resource="http://purl.obolibrary.org/obo/UO_1000218"/>
        <oboInOwl:hasExactSynonym>MV</oboInOwl:hasExactSynonym>
        <rdfs:comment>&quot;An electric potential difference unit which is equal to one million volts or 10^[6] V.&quot; [UOC:GVG]</rdfs:comment>
        <rdfs:label>megavolt</rdfs:label>
    </owl:Class>
    


    <!-- http://purl.obolibrary.org/obo/UO_0000261 -->

    <owl:Class rdf:about="http://purl.obolibrary.org/obo/UO_0000261">
        <rdfs:subClassOf rdf:resource="http://purl.obolibrary.org/obo/UO_0000000"/>
        <rdfs:comment>&quot;A unit which represents a standard measurement of the transmission of an entity through a medium.&quot; [UOC:GVG]</rdfs:comment>
        <rdfs:label>conduction unit</rdfs:label>
    </owl:Class>
    


    <!-- http://purl.obolibrary.org/obo/UO_0000262 -->

    <owl:Class rdf:about="http://purl.obolibrary.org/obo/UO_0000262">
        <rdfs:subClassOf rdf:resource="http://purl.obolibrary.org/obo/UO_0000261"/>
        <rdfs:comment>&quot;A unit which represents a standard measurement of the movement of electrically charged particles through a transmission medium (electrical conductor).&quot; [UOC:GVG]</rdfs:comment>
        <rdfs:label>electrical conduction unit</rdfs:label>
    </owl:Class>
    


    <!-- http://purl.obolibrary.org/obo/UO_0000264 -->

    <owl:Class rdf:about="http://purl.obolibrary.org/obo/UO_0000264">
        <rdfs:subClassOf rdf:resource="http://purl.obolibrary.org/obo/UO_1000264"/>
        <oboInOwl:hasExactSynonym>A V^-1</oboInOwl:hasExactSynonym>
        <oboInOwl:hasExactSynonym>mho </oboInOwl:hasExactSynonym>
        <oboInOwl:hasRelatedSynonym>S</oboInOwl:hasRelatedSynonym>
        <rdfs:comment>&quot;An electrical conduction unit which is equal to A/V.&quot; [NIST:NIST]</rdfs:comment>
        <rdfs:label>siemens</rdfs:label>
    </owl:Class>
    


    <!-- http://purl.obolibrary.org/obo/UO_0000270 -->

    <owl:Class rdf:about="http://purl.obolibrary.org/obo/UO_0000270">
        <rdfs:subClassOf rdf:resource="http://purl.obolibrary.org/obo/UO_0000000"/>
        <rdfs:comment>&quot;A unit which is a standard measure of the volume of fluid which passes through a given surface per unit time .&quot; [Wikipedia:Wikipedia]</rdfs:comment>
        <rdfs:label>volumetric flow rate unit</rdfs:label>
    </owl:Class>
    


    <!-- http://purl.obolibrary.org/obo/UO_0000280 -->

    <owl:Class rdf:about="http://purl.obolibrary.org/obo/UO_0000280">
        <rdfs:subClassOf rdf:resource="http://purl.obolibrary.org/obo/UO_0000000"/>
        <rdfs:comment>&quot;A unit which represents a standard measurement occurrence of a process per unit time.&quot; [UOC:GVG]</rdfs:comment>
        <rdfs:label>rate unit</rdfs:label>
    </owl:Class>
    


    <!-- http://purl.obolibrary.org/obo/UO_0000286 -->

    <owl:Class rdf:about="http://purl.obolibrary.org/obo/UO_0000286">
        <rdfs:subClassOf rdf:resource="http://purl.obolibrary.org/obo/UO_0000046"/>
        <oboInOwl:hasExactSynonym>10^[24]</oboInOwl:hasExactSynonym>
        <oboInOwl:hasExactSynonym>Y</oboInOwl:hasExactSynonym>
        <rdfs:comment>&quot;A prefix in the metric system denoting a factor of ten to the power of 24.&quot; [UO:GVG]</rdfs:comment>
        <rdfs:label>yotta</rdfs:label>
    </owl:Class>
    


    <!-- http://purl.obolibrary.org/obo/UO_0000287 -->

    <owl:Class rdf:about="http://purl.obolibrary.org/obo/UO_0000287">
        <rdfs:subClassOf rdf:resource="http://purl.obolibrary.org/obo/UO_0000046"/>
        <oboInOwl:hasExactSynonym>10^[2]</oboInOwl:hasExactSynonym>
        <oboInOwl:hasExactSynonym>h</oboInOwl:hasExactSynonym>
        <rdfs:comment>&quot;A prefix in the metric system denoting a factor of one hundred.&quot; [UO:GVG]</rdfs:comment>
        <rdfs:label>hecto</rdfs:label>
    </owl:Class>
    


    <!-- http://purl.obolibrary.org/obo/UO_0000288 -->

    <owl:Class rdf:about="http://purl.obolibrary.org/obo/UO_0000288">
        <rdfs:subClassOf rdf:resource="http://purl.obolibrary.org/obo/UO_0000046"/>
        <oboInOwl:hasExactSynonym>10^[21]</oboInOwl:hasExactSynonym>
        <oboInOwl:hasExactSynonym>Z</oboInOwl:hasExactSynonym>
        <rdfs:comment>&quot;A prefix in the metric system denoting a factor of ten to the power of 21.&quot; [UO:GVG]</rdfs:comment>
        <rdfs:label>zetta</rdfs:label>
    </owl:Class>
    


    <!-- http://purl.obolibrary.org/obo/UO_0000289 -->

    <owl:Class rdf:about="http://purl.obolibrary.org/obo/UO_0000289">
        <rdfs:subClassOf rdf:resource="http://purl.obolibrary.org/obo/UO_0000046"/>
        <oboInOwl:hasExactSynonym>10^[18]</oboInOwl:hasExactSynonym>
        <oboInOwl:hasExactSynonym>E</oboInOwl:hasExactSynonym>
        <rdfs:comment>&quot;A prefix in the metric system denoting a factor of ten to the power of 18.&quot; [UO:GVG]</rdfs:comment>
        <rdfs:label>exa</rdfs:label>
    </owl:Class>
    


    <!-- http://purl.obolibrary.org/obo/UO_0000290 -->

    <owl:Class rdf:about="http://purl.obolibrary.org/obo/UO_0000290">
        <rdfs:subClassOf rdf:resource="http://purl.obolibrary.org/obo/UO_0000046"/>
        <oboInOwl:hasExactSynonym>10^[15]</oboInOwl:hasExactSynonym>
        <oboInOwl:hasExactSynonym>P</oboInOwl:hasExactSynonym>
        <rdfs:comment>&quot;A prefix in the metric system denoting a factor of ten to the power of 15.&quot; [UO:GVG]</rdfs:comment>
        <rdfs:label>peta</rdfs:label>
    </owl:Class>
    


    <!-- http://purl.obolibrary.org/obo/UO_0000291 -->

    <owl:Class rdf:about="http://purl.obolibrary.org/obo/UO_0000291">
        <rdfs:subClassOf rdf:resource="http://purl.obolibrary.org/obo/UO_0000046"/>
        <oboInOwl:hasExactSynonym>T</oboInOwl:hasExactSynonym>
        <oboInOwl:hasRelatedSynonym>10^[12]</oboInOwl:hasRelatedSynonym>
        <rdfs:comment>&quot;A prefix in the metric system denoting a factor of ten to the power of 12.&quot; [UO:GVG]</rdfs:comment>
        <rdfs:label>tera</rdfs:label>
    </owl:Class>
    


    <!-- http://purl.obolibrary.org/obo/UO_0000292 -->

    <owl:Class rdf:about="http://purl.obolibrary.org/obo/UO_0000292">
        <rdfs:subClassOf rdf:resource="http://purl.obolibrary.org/obo/UO_0000046"/>
        <oboInOwl:hasExactSynonym>10^[9]</oboInOwl:hasExactSynonym>
        <oboInOwl:hasExactSynonym>G</oboInOwl:hasExactSynonym>
        <rdfs:comment>&quot;A prefix in the metric system denoting a factor of ten to the power of 9.&quot; [UO:GVG]</rdfs:comment>
        <rdfs:label>giga</rdfs:label>
    </owl:Class>
    


    <!-- http://purl.obolibrary.org/obo/UO_0000293 -->

    <owl:Class rdf:about="http://purl.obolibrary.org/obo/UO_0000293">
        <rdfs:subClassOf rdf:resource="http://purl.obolibrary.org/obo/UO_0000046"/>
        <oboInOwl:hasExactSynonym>10^[6]</oboInOwl:hasExactSynonym>
        <oboInOwl:hasExactSynonym>M</oboInOwl:hasExactSynonym>
        <rdfs:comment>&quot;A prefix in the metric system denoting a factor of million.&quot; [UO:GVG]</rdfs:comment>
        <rdfs:label>mega</rdfs:label>
    </owl:Class>
    


    <!-- http://purl.obolibrary.org/obo/UO_0000294 -->

    <owl:Class rdf:about="http://purl.obolibrary.org/obo/UO_0000294">
        <rdfs:subClassOf rdf:resource="http://purl.obolibrary.org/obo/UO_0000046"/>
        <oboInOwl:hasExactSynonym>10^[3]</oboInOwl:hasExactSynonym>
        <oboInOwl:hasExactSynonym>k</oboInOwl:hasExactSynonym>
        <rdfs:comment>&quot;A prefix in the metric system denoting a factor of one thousand.&quot; [UO:GVG]</rdfs:comment>
        <rdfs:label>kilo</rdfs:label>
    </owl:Class>
    


    <!-- http://purl.obolibrary.org/obo/UO_0000295 -->

    <owl:Class rdf:about="http://purl.obolibrary.org/obo/UO_0000295">
        <rdfs:subClassOf rdf:resource="http://purl.obolibrary.org/obo/UO_0000046"/>
        <oboInOwl:hasExactSynonym>10^[1]</oboInOwl:hasExactSynonym>
        <oboInOwl:hasExactSynonym>da</oboInOwl:hasExactSynonym>
        <rdfs:comment>&quot;A prefix in the metric system denoting a factor of ten.&quot; [UO:GVG]</rdfs:comment>
        <rdfs:label>deca</rdfs:label>
    </owl:Class>
    


    <!-- http://purl.obolibrary.org/obo/UO_0000297 -->

    <owl:Class rdf:about="http://purl.obolibrary.org/obo/UO_0000297">
        <rdfs:subClassOf rdf:resource="http://purl.obolibrary.org/obo/UO_0000046"/>
        <oboInOwl:hasExactSynonym>10^[-3]</oboInOwl:hasExactSynonym>
        <oboInOwl:hasExactSynonym>m</oboInOwl:hasExactSynonym>
        <rdfs:comment>&quot;A prefix in the metric system denoting a factor of one thousand.&quot; [UO:GVG]</rdfs:comment>
        <rdfs:label>milli</rdfs:label>
    </owl:Class>
    


    <!-- http://purl.obolibrary.org/obo/UO_0000298 -->

    <owl:Class rdf:about="http://purl.obolibrary.org/obo/UO_0000298">
        <rdfs:subClassOf rdf:resource="http://purl.obolibrary.org/obo/UO_0000046"/>
        <oboInOwl:hasExactSynonym>10^[-2]</oboInOwl:hasExactSynonym>
        <oboInOwl:hasExactSynonym>c</oboInOwl:hasExactSynonym>
        <rdfs:comment>&quot;A prefix in the metric system denoting a factor of one hundred.&quot; [UO:GVG]</rdfs:comment>
        <rdfs:label>centi</rdfs:label>
    </owl:Class>
    


    <!-- http://purl.obolibrary.org/obo/UO_0000299 -->

    <owl:Class rdf:about="http://purl.obolibrary.org/obo/UO_0000299">
        <rdfs:subClassOf rdf:resource="http://purl.obolibrary.org/obo/UO_0000046"/>
        <oboInOwl:hasExactSynonym>10^[-6]</oboInOwl:hasExactSynonym>
        <rdfs:comment>&quot;A prefix in the metric system denoting a factor of 10 to the power of -6.&quot; [UO:GVG]</rdfs:comment>
        <rdfs:label>micro</rdfs:label>
    </owl:Class>
    


    <!-- http://purl.obolibrary.org/obo/UO_0000300 -->

    <owl:Class rdf:about="http://purl.obolibrary.org/obo/UO_0000300">
        <rdfs:subClassOf rdf:resource="http://purl.obolibrary.org/obo/UO_0000046"/>
        <oboInOwl:hasExactSynonym>10^[-9]</oboInOwl:hasExactSynonym>
        <oboInOwl:hasExactSynonym>n</oboInOwl:hasExactSynonym>
        <rdfs:comment>&quot;A prefix in the metric system denoting a factor of 10 to the power of -9.&quot; [UO:GVG]</rdfs:comment>
        <rdfs:label>nano</rdfs:label>
    </owl:Class>
    


    <!-- http://purl.obolibrary.org/obo/UO_0000302 -->

    <owl:Class rdf:about="http://purl.obolibrary.org/obo/UO_0000302">
        <rdfs:subClassOf rdf:resource="http://purl.obolibrary.org/obo/UO_0000046"/>
        <oboInOwl:hasExactSynonym>10^[-12]</oboInOwl:hasExactSynonym>
        <oboInOwl:hasExactSynonym>n</oboInOwl:hasExactSynonym>
        <rdfs:comment>&quot;A prefix in the metric system denoting a factor of 10 to the power of -12.&quot; [GVG:UO]</rdfs:comment>
        <rdfs:label>pico</rdfs:label>
    </owl:Class>
    


    <!-- http://purl.obolibrary.org/obo/UO_0000303 -->

    <owl:Class rdf:about="http://purl.obolibrary.org/obo/UO_0000303">
        <rdfs:subClassOf rdf:resource="http://purl.obolibrary.org/obo/UO_0000046"/>
        <oboInOwl:hasExactSynonym>10^[-15]</oboInOwl:hasExactSynonym>
        <oboInOwl:hasExactSynonym>f</oboInOwl:hasExactSynonym>
        <rdfs:comment>&quot;A prefix in the metric system denoting a factor of 10 to the power of -15.&quot; [UO:GVG]</rdfs:comment>
        <rdfs:label>femto</rdfs:label>
    </owl:Class>
    


    <!-- http://purl.obolibrary.org/obo/UO_0000304 -->

    <owl:Class rdf:about="http://purl.obolibrary.org/obo/UO_0000304">
        <rdfs:subClassOf rdf:resource="http://purl.obolibrary.org/obo/UO_0000046"/>
        <oboInOwl:hasExactSynonym>a</oboInOwl:hasExactSynonym>
        <oboInOwl:hasRelatedSynonym>10^[-18]</oboInOwl:hasRelatedSynonym>
        <rdfs:comment>&quot;A prefix in the metric system denoting a factor of 10 to the power of -18.&quot; [UO:GVG]</rdfs:comment>
        <rdfs:label>atto</rdfs:label>
    </owl:Class>
    


    <!-- http://purl.obolibrary.org/obo/UO_0000305 -->

    <owl:Class rdf:about="http://purl.obolibrary.org/obo/UO_0000305">
        <rdfs:subClassOf rdf:resource="http://purl.obolibrary.org/obo/UO_0000046"/>
        <oboInOwl:hasExactSynonym>z</oboInOwl:hasExactSynonym>
        <oboInOwl:hasRelatedSynonym>10^[-21]</oboInOwl:hasRelatedSynonym>
        <rdfs:comment>&quot;A prefix in the metric system denoting a factor of 10 to the power of -21.&quot; [UO:GVG]</rdfs:comment>
        <rdfs:label>zepto</rdfs:label>
    </owl:Class>
    


    <!-- http://purl.obolibrary.org/obo/UO_0000306 -->

    <owl:Class rdf:about="http://purl.obolibrary.org/obo/UO_0000306">
        <rdfs:subClassOf rdf:resource="http://purl.obolibrary.org/obo/UO_0000046"/>
        <oboInOwl:hasExactSynonym>y</oboInOwl:hasExactSynonym>
        <oboInOwl:hasRelatedSynonym>10^[-24]</oboInOwl:hasRelatedSynonym>
        <rdfs:comment>&quot;A prefix in the metric system denoting a factor of 10 to the power of -24.&quot; [UO:GVG]</rdfs:comment>
        <rdfs:label>yocto</rdfs:label>
    </owl:Class>
    


    <!-- http://purl.obolibrary.org/obo/UO_0000325 -->

    <owl:Class rdf:about="http://purl.obolibrary.org/obo/UO_0000325">
        <rdfs:subClassOf rdf:resource="http://purl.obolibrary.org/obo/UO_0000105"/>
        <oboInOwl:hasRelatedSynonym>mH</oboInOwl:hasRelatedSynonym>
        <oboInOwl:hasRelatedSynonym>megahertz</oboInOwl:hasRelatedSynonym>
        <rdfs:comment>&quot;A frequency unit which is equal to one million hertz or 10^[6] V.&quot; [UOC:GVG]</rdfs:comment>
        <rdfs:label>megaHertz</rdfs:label>
    </owl:Class>
    


    <!-- http://purl.obolibrary.org/obo/UO_0000331 -->

    <owl:Class rdf:about="http://purl.obolibrary.org/obo/UO_0000331">
        <rdfs:subClassOf rdf:resource="http://purl.obolibrary.org/obo/UO_0000231"/>
        <oboInOwl:hasExactSynonym>GB</oboInOwl:hasExactSynonym>
        <rdfs:comment>&quot;An information unit which is equal to 1000000000 bytes.&quot; [UO:GVG]</rdfs:comment>
        <rdfs:label>gigabyte</rdfs:label>
    </owl:Class>
    


    <!-- http://purl.obolibrary.org/obo/UO_0000332 -->

    <owl:Class rdf:about="http://purl.obolibrary.org/obo/UO_0000332">
        <rdfs:subClassOf rdf:resource="http://purl.obolibrary.org/obo/UO_0000231"/>
        <oboInOwl:hasExactSynonym>TB</oboInOwl:hasExactSynonym>
        <rdfs:comment>&quot;An information unit which is equal to 1000 gigabytes.&quot; [UO:GVG]</rdfs:comment>
        <rdfs:label>terabyte</rdfs:label>
    </owl:Class>
    


    <!-- http://purl.obolibrary.org/obo/UO_0010006 -->

    <owl:Class rdf:about="http://purl.obolibrary.org/obo/UO_0010006">
        <rdfs:subClassOf rdf:resource="http://purl.obolibrary.org/obo/UO_0000190"/>
        <rdfs:comment>&quot;A dimensionless ratio unit which, given a pair of quantities a and b, for which b is a multiple of a, denotes b by giving the multiplier (coefficient) c for a to result in b.&quot; [UOB:LKSR]</rdfs:comment>
        <rdfs:label>ratio</rdfs:label>
    </owl:Class>
    


    <!-- http://purl.obolibrary.org/obo/UO_0010008 -->

    <owl:Class rdf:about="http://purl.obolibrary.org/obo/UO_0010008">
        <rdfs:subClassOf rdf:resource="http://purl.obolibrary.org/obo/UO_0000060"/>
        <oboInOwl:hasExactSynonym>kilometre per hour</oboInOwl:hasExactSynonym>
        <oboInOwl:hasExactSynonym>km/h</oboInOwl:hasExactSynonym>
        <rdfs:comment>&quot;A speed/velocity unit which is equal to the speed of an object traveling 1 kilometer distance in one hour.&quot; [NIST:NIST]</rdfs:comment>
        <rdfs:label>kilometer per hour</rdfs:label>
    </owl:Class>
    


    <!-- http://purl.obolibrary.org/obo/UO_0010010 -->

    <owl:Class rdf:about="http://purl.obolibrary.org/obo/UO_0010010">
        <rdfs:subClassOf rdf:resource="http://purl.obolibrary.org/obo/UO_1010010"/>
        <oboInOwl:hasExactSynonym>HA</oboInOwl:hasExactSynonym>
        <rdfs:comment>&quot;An area unit which is equal to an area of 10,000 square meters. Equivalent to 2.471 acres.&quot; [Wikipedia:Wikipedia]</rdfs:comment>
        <rdfs:label>hectare</rdfs:label>
    </owl:Class>
    


    <!-- http://purl.obolibrary.org/obo/UO_0010066 -->

    <owl:Class rdf:about="http://purl.obolibrary.org/obo/UO_0010066">
        <rdfs:subClassOf rdf:resource="http://purl.obolibrary.org/obo/UO_1000008"/>
        <oboInOwl:hasExactSynonym>kilometre</oboInOwl:hasExactSynonym>
        <oboInOwl:hasExactSynonym>km</oboInOwl:hasExactSynonym>
        <rdfs:comment>&quot;A length unit which is equal to one thousand meters.&quot; [UOB:LKSR]</rdfs:comment>
        <rdfs:label>kilometer</rdfs:label>
    </owl:Class>
    


    <!-- http://purl.obolibrary.org/obo/UO_1000008 -->

    <owl:Class rdf:about="http://purl.obolibrary.org/obo/UO_1000008">
        <rdfs:subClassOf rdf:resource="http://purl.obolibrary.org/obo/UO_0000001"/>
        <rdfs:label>meter based unit</rdfs:label>
    </owl:Class>
    


    <!-- http://purl.obolibrary.org/obo/UO_1000010 -->

    <owl:Class rdf:about="http://purl.obolibrary.org/obo/UO_1000010">
        <rdfs:subClassOf rdf:resource="http://purl.obolibrary.org/obo/UO_0000003"/>
        <rdfs:label>second based unit</rdfs:label>
    </owl:Class>
    


    <!-- http://purl.obolibrary.org/obo/UO_1000011 -->

    <owl:Class rdf:about="http://purl.obolibrary.org/obo/UO_1000011">
        <rdfs:subClassOf rdf:resource="http://purl.obolibrary.org/obo/UO_0000004"/>
        <rdfs:label>ampere based unit</rdfs:label>
    </owl:Class>
    


    <!-- http://purl.obolibrary.org/obo/UO_1000012 -->

    <owl:Class rdf:about="http://purl.obolibrary.org/obo/UO_1000012">
        <rdfs:subClassOf rdf:resource="http://purl.obolibrary.org/obo/UO_0000005"/>
        <rdfs:label>kelvin based unit</rdfs:label>
    </owl:Class>
    


    <!-- http://purl.obolibrary.org/obo/UO_1000014 -->

    <owl:Class rdf:about="http://purl.obolibrary.org/obo/UO_1000014">
        <rdfs:subClassOf rdf:resource="http://purl.obolibrary.org/obo/UO_0000007"/>
        <rdfs:label>candela based unit</rdfs:label>
    </owl:Class>
    


    <!-- http://purl.obolibrary.org/obo/UO_1000021 -->

    <owl:Class rdf:about="http://purl.obolibrary.org/obo/UO_1000021">
        <rdfs:subClassOf rdf:resource="http://purl.obolibrary.org/obo/UO_0000002"/>
        <rdfs:label>gram based unit</rdfs:label>
    </owl:Class>
    


    <!-- http://purl.obolibrary.org/obo/UO_1000027 -->

    <owl:Class rdf:about="http://purl.obolibrary.org/obo/UO_1000027">
        <rdfs:subClassOf rdf:resource="http://purl.obolibrary.org/obo/UO_0000005"/>
        <rdfs:label>degree Celsius based unit</rdfs:label>
    </owl:Class>
    


    <!-- http://purl.obolibrary.org/obo/UO_1000031 -->

    <owl:Class rdf:about="http://purl.obolibrary.org/obo/UO_1000031">
        <rdfs:subClassOf rdf:resource="http://purl.obolibrary.org/obo/UO_0000003"/>
        <rdfs:label>minute based unit</rdfs:label>
    </owl:Class>
    


    <!-- http://purl.obolibrary.org/obo/UO_1000032 -->

    <owl:Class rdf:about="http://purl.obolibrary.org/obo/UO_1000032">
        <rdfs:subClassOf rdf:resource="http://purl.obolibrary.org/obo/UO_0000003"/>
        <rdfs:label>hour based unit</rdfs:label>
    </owl:Class>
    


    <!-- http://purl.obolibrary.org/obo/UO_1000033 -->

    <owl:Class rdf:about="http://purl.obolibrary.org/obo/UO_1000033">
        <rdfs:subClassOf rdf:resource="http://purl.obolibrary.org/obo/UO_0000003"/>
        <rdfs:label>day based unit</rdfs:label>
    </owl:Class>
    


    <!-- http://purl.obolibrary.org/obo/UO_1000034 -->

    <owl:Class rdf:about="http://purl.obolibrary.org/obo/UO_1000034">
        <rdfs:subClassOf rdf:resource="http://purl.obolibrary.org/obo/UO_0000003"/>
        <rdfs:label>week based unit</rdfs:label>
    </owl:Class>
    


    <!-- http://purl.obolibrary.org/obo/UO_1000035 -->

    <owl:Class rdf:about="http://purl.obolibrary.org/obo/UO_1000035">
        <rdfs:subClassOf rdf:resource="http://purl.obolibrary.org/obo/UO_0000003"/>
        <rdfs:label>month based unit</rdfs:label>
    </owl:Class>
    


    <!-- http://purl.obolibrary.org/obo/UO_1000036 -->

    <owl:Class rdf:about="http://purl.obolibrary.org/obo/UO_1000036">
        <rdfs:subClassOf rdf:resource="http://purl.obolibrary.org/obo/UO_0000003"/>
        <rdfs:label>year based unit</rdfs:label>
    </owl:Class>
    


    <!-- http://purl.obolibrary.org/obo/UO_1000080 -->

    <owl:Class rdf:about="http://purl.obolibrary.org/obo/UO_1000080">
        <rdfs:subClassOf rdf:resource="http://purl.obolibrary.org/obo/UO_0000047"/>
        <rdfs:label>square meter based unit</rdfs:label>
    </owl:Class>
    


    <!-- http://purl.obolibrary.org/obo/UO_1000082 -->

    <owl:Class rdf:about="http://purl.obolibrary.org/obo/UO_1000082">
        <rdfs:subClassOf rdf:resource="http://purl.obolibrary.org/obo/UO_0000047"/>
        <rdfs:label>square millimeter based unit</rdfs:label>
    </owl:Class>
    


    <!-- http://purl.obolibrary.org/obo/UO_1000092 -->

    <owl:Class rdf:about="http://purl.obolibrary.org/obo/UO_1000092">
        <rdfs:subClassOf rdf:resource="http://purl.obolibrary.org/obo/UO_0000058"/>
        <rdfs:label>turns per second based unit</rdfs:label>
    </owl:Class>
    


    <!-- http://purl.obolibrary.org/obo/UO_1000094 -->

    <owl:Class rdf:about="http://purl.obolibrary.org/obo/UO_1000094">
        <rdfs:subClassOf rdf:resource="http://purl.obolibrary.org/obo/UO_0000060"/>
        <rdfs:label>meter per second based unit</rdfs:label>
    </owl:Class>
    


    <!-- http://purl.obolibrary.org/obo/UO_1000096 -->

    <owl:Class rdf:about="http://purl.obolibrary.org/obo/UO_1000096">
        <rdfs:subClassOf rdf:resource="http://purl.obolibrary.org/obo/UO_0000095"/>
        <rdfs:label>cubic meter based unit</rdfs:label>
    </owl:Class>
    


    <!-- http://purl.obolibrary.org/obo/UO_1000097 -->

    <owl:Class rdf:about="http://purl.obolibrary.org/obo/UO_1000097">
        <rdfs:subClassOf rdf:resource="http://purl.obolibrary.org/obo/UO_0000095"/>
        <rdfs:label>cubic centimeter based unit</rdfs:label>
    </owl:Class>
    


    <!-- http://purl.obolibrary.org/obo/UO_1000099 -->

    <owl:Class rdf:about="http://purl.obolibrary.org/obo/UO_1000099">
        <rdfs:subClassOf rdf:resource="http://purl.obolibrary.org/obo/UO_0000095"/>
        <rdfs:label>liter based unit</rdfs:label>
    </owl:Class>
    


    <!-- http://purl.obolibrary.org/obo/UO_1000106 -->

    <owl:Class rdf:about="http://purl.obolibrary.org/obo/UO_1000106">
        <rdfs:subClassOf rdf:resource="http://purl.obolibrary.org/obo/UO_0000105"/>
        <rdfs:label>hertz based unit</rdfs:label>
    </owl:Class>
    


    <!-- http://purl.obolibrary.org/obo/UO_1000108 -->

    <owl:Class rdf:about="http://purl.obolibrary.org/obo/UO_1000108">
        <rdfs:subClassOf rdf:resource="http://purl.obolibrary.org/obo/UO_0000107"/>
        <rdfs:label>newton based unit</rdfs:label>
    </owl:Class>
    


    <!-- http://purl.obolibrary.org/obo/UO_1000110 -->

    <owl:Class rdf:about="http://purl.obolibrary.org/obo/UO_1000110">
        <rdfs:subClassOf rdf:resource="http://purl.obolibrary.org/obo/UO_0000109"/>
        <rdfs:label>pascal based unit</rdfs:label>
    </owl:Class>
    


    <!-- http://purl.obolibrary.org/obo/UO_1000112 -->

    <owl:Class rdf:about="http://purl.obolibrary.org/obo/UO_1000112">
        <rdfs:subClassOf rdf:resource="http://purl.obolibrary.org/obo/UO_0000111"/>
        <rdfs:label>joule based unit</rdfs:label>
    </owl:Class>
    


    <!-- http://purl.obolibrary.org/obo/UO_1000114 -->

    <owl:Class rdf:about="http://purl.obolibrary.org/obo/UO_1000114">
        <rdfs:subClassOf rdf:resource="http://purl.obolibrary.org/obo/UO_0000113"/>
        <rdfs:label>watt based unit</rdfs:label>
    </owl:Class>
    


    <!-- http://purl.obolibrary.org/obo/UO_1000116 -->

    <owl:Class rdf:about="http://purl.obolibrary.org/obo/UO_1000116">
        <rdfs:subClassOf rdf:resource="http://purl.obolibrary.org/obo/UO_0000115"/>
        <rdfs:label>lux based unit</rdfs:label>
    </owl:Class>
    


    <!-- http://purl.obolibrary.org/obo/UO_1000118 -->

    <owl:Class rdf:about="http://purl.obolibrary.org/obo/UO_1000118">
        <rdfs:subClassOf rdf:resource="http://purl.obolibrary.org/obo/UO_0000117"/>
        <rdfs:label>lumen based unit</rdfs:label>
    </owl:Class>
    


    <!-- http://purl.obolibrary.org/obo/UO_1000123 -->

    <owl:Class rdf:about="http://purl.obolibrary.org/obo/UO_1000123">
        <rdfs:subClassOf rdf:resource="http://purl.obolibrary.org/obo/UO_0000122"/>
        <rdfs:label>radian based unit</rdfs:label>
    </owl:Class>
    


    <!-- http://purl.obolibrary.org/obo/UO_1000155 -->

    <owl:Class rdf:about="http://purl.obolibrary.org/obo/UO_1000155">
        <rdfs:subClassOf rdf:resource="http://purl.obolibrary.org/obo/UO_0000154"/>
        <rdfs:label>watt per square meter based unit</rdfs:label>
    </owl:Class>
    


    <!-- http://purl.obolibrary.org/obo/UO_1000169 -->

    <owl:Class rdf:about="http://purl.obolibrary.org/obo/UO_1000169">
        <rdfs:subClassOf rdf:resource="http://purl.obolibrary.org/obo/UO_0000166"/>
        <rdfs:label>parts per million based unit</rdfs:label>
    </owl:Class>
    


    <!-- http://purl.obolibrary.org/obo/UO_1000185 -->

    <owl:Class rdf:about="http://purl.obolibrary.org/obo/UO_1000185">
        <rdfs:subClassOf rdf:resource="http://purl.obolibrary.org/obo/UO_0000122"/>
        <rdfs:label>degree based unit</rdfs:label>
    </owl:Class>
    


    <!-- http://purl.obolibrary.org/obo/UO_1000188 -->

    <owl:Class rdf:about="http://purl.obolibrary.org/obo/UO_1000188">
        <rdfs:subClassOf rdf:resource="http://purl.obolibrary.org/obo/UO_0000186"/>
        <rdfs:label>pi based unit</rdfs:label>
    </owl:Class>
    


    <!-- http://purl.obolibrary.org/obo/UO_1000196 -->

    <owl:Class rdf:about="http://purl.obolibrary.org/obo/UO_1000196">
        <rdfs:subClassOf rdf:resource="http://purl.obolibrary.org/obo/UO_0000051"/>
        <rdfs:subClassOf rdf:resource="http://purl.obolibrary.org/obo/UO_0000186"/>
        <rdfs:label>pH based unit</rdfs:label>
    </owl:Class>
    


    <!-- http://purl.obolibrary.org/obo/UO_1000218 -->

    <owl:Class rdf:about="http://purl.obolibrary.org/obo/UO_1000218">
        <rdfs:subClassOf rdf:resource="http://purl.obolibrary.org/obo/UO_0000217"/>
        <rdfs:label>volt based unit</rdfs:label>
    </owl:Class>
    


    <!-- http://purl.obolibrary.org/obo/UO_1000220 -->

    <owl:Class rdf:about="http://purl.obolibrary.org/obo/UO_1000220">
        <rdfs:subClassOf rdf:resource="http://purl.obolibrary.org/obo/UO_0000219"/>
        <rdfs:label>coulomb based unit</rdfs:label>
    </owl:Class>
    


    <!-- http://purl.obolibrary.org/obo/UO_1000223 -->

    <owl:Class rdf:about="http://purl.obolibrary.org/obo/UO_1000223">
        <rdfs:subClassOf rdf:resource="http://purl.obolibrary.org/obo/UO_0000111"/>
        <rdfs:label>watt-hour based unit</rdfs:label>
    </owl:Class>
    


    <!-- http://purl.obolibrary.org/obo/UO_1000232 -->

    <owl:Class rdf:about="http://purl.obolibrary.org/obo/UO_1000232">
        <rdfs:subClassOf rdf:resource="http://purl.obolibrary.org/obo/UO_0000231"/>
        <rdfs:label>bit based unit</rdfs:label>
    </owl:Class>
    


    <!-- http://purl.obolibrary.org/obo/UO_1000233 -->

    <owl:Class rdf:about="http://purl.obolibrary.org/obo/UO_1000233">
        <rdfs:subClassOf rdf:resource="http://purl.obolibrary.org/obo/UO_0000231"/>
        <rdfs:label>byte based unit</rdfs:label>
    </owl:Class>
    


    <!-- http://purl.obolibrary.org/obo/UO_1000264 -->

    <owl:Class rdf:about="http://purl.obolibrary.org/obo/UO_1000264">
        <rdfs:subClassOf rdf:resource="http://purl.obolibrary.org/obo/UO_0000262"/>
        <rdfs:label>siemens based unit</rdfs:label>
    </owl:Class>
    


    <!-- http://purl.obolibrary.org/obo/UO_1010010 -->

    <owl:Class rdf:about="http://purl.obolibrary.org/obo/UO_1010010">
        <rdfs:subClassOf rdf:resource="http://purl.obolibrary.org/obo/UO_0000047"/>
        <rdfs:label>hectare based unit</rdfs:label>
    </owl:Class>
    


    <!-- http://purl.obolibrary.org/obo/UO_1010049 -->

    <owl:Class rdf:about="http://purl.obolibrary.org/obo/UO_1010049">
        <rdfs:subClassOf rdf:resource="http://purl.obolibrary.org/obo/UO_0000054"/>
        <rdfs:label>gram per square meter based unit</rdfs:label>
    </owl:Class>
</rdf:RDF>



<!-- Generated by the OWL API (version 4.5.25) https://github.com/owlcs/owlapi -->

